Deadcode proof

backend/Deadcode.v
@@ -217,3 +217,175 @@ Definition transf_fundef (rm: romem) (fd: fundef) : res fundef :=
 Definition transf_program (p: program) : res program :=
   transform_partial_program (transf_fundef (romem_for p)) p.
 
+
+Inductive match_nmem_alpha (a:permutation) : nmem -> nmem -> Prop :=
+| match_nmem_dead : match_nmem_alpha a NMemDead NMemDead
+| match_nmem_used : forall stk1 stk2 gl1 gl2,
+    IntvSets.ISet.beq stk1 stk2 = true ->
+    (forall id, match_option_alpha a (fun _ intv1 intv2 => IntvSets.ISet.beq intv1 intv2 = true)  (gl1 ! (alpha_rename a id)) (gl2 ! id)) ->
+    match_nmem_alpha a (NMem stk1 gl1) (NMem stk2 gl2).
+
+
+Definition match_NA_alpha (a:permutation) (na1 na2: NA.t) :=
+  PTree.beq eq_nval (fst na1) (fst na2) = true /\
+  match_nmem_alpha a (snd na2) (snd na2).
+
+Lemma Deadcode_analyze_alpha: forall a f pva1 pva2,
+    (forall pc, match_VA_alpha a pva1!!pc pva2!!pc) ->
+     match_option_alpha a (fun a pn1 pn2 => forall pc, match_NA_alpha a pn1!!pc pn2!!pc) (analyze pva1 (alpha_rename a f)) (analyze pva2 f).
+Admitted.
+
+Lemma is_dead_alpha: forall a pn1 pn2 node r,
+      (forall pc : positive, match_NA_alpha a pn1 # pc pn2 # pc) ->
+      is_dead (nreg (fst pn1#node) r) = is_dead (nreg (fst pn2#node) r).
+Admitted.
+
+Lemma is_int_zero_alpha: forall a pn1 pn2 node r,
+      (forall pc : positive, match_NA_alpha a pn1 # pc pn2 # pc) ->
+      is_int_zero (nreg (fst pn1#node) r) = is_int_zero (nreg (fst pn2#node) r).
+  Admitted.
+
+Lemma operation_is_redundant_alpha: forall a pn1 pn2 node r op,
+    (forall pc : positive, match_NA_alpha a pn1 # pc pn2 # pc) ->
+    operation_is_redundant (alpha_rename a op) (nreg (fst pn1#node) r) = operation_is_redundant op (nreg (fst pn2#node) r).
+Admitted.
+
+Lemma aaddressing_alpha: forall a va1 va2 addr l,
+    match_VA_alpha a va1 va2 ->
+    aaddressing va1 (alpha_rename a addr) l = alpha_rename a (aaddressing va2 addr l).
+Admitted.
+
+Lemma aaddr_arg_alpha: forall a va1 va2 arg,
+    match_VA_alpha a va1 va2 ->
+    aaddr_arg va1 (alpha_rename a arg) = alpha_rename a (aaddr_arg va2 arg).
+Admitted.
+
+
+Lemma nmem_contains_alpha: forall a pva1 pva2 pn1 pn2 node ap size,
+      (forall pc : positive, match_VA_alpha a pva1 # pc pva2 # pc) ->
+      (forall pc : positive, match_NA_alpha a pn1 # pc pn2 # pc) ->
+      nmem_contains (snd pn1 # node) (alpha_rename a ap) size = nmem_contains (snd pn2#node) ap size.
+Admitted.
+    
+
+Lemma transf_instr_alpha : forall a pva1 pva2 pn1 pn2 i node,
+    (forall pc : positive, match_VA_alpha a pva1 !! pc pva2 !! pc) ->
+    (forall pc : positive, match_NA_alpha a pn1 !! pc pn2 !! pc) ->
+    transf_instr pva1 pn1 node (alpha_rename a i) =
+    alpha_rename a (transf_instr pva2 pn2 node i).
+Proof.
+  intros.
+  Transparent Alpha_instruction.
+  destruct i;simpl;auto.
+  - generalize (is_dead_alpha _ _ _ node r H0).
+    intros. rewrite H1. destruct (is_dead (nreg (fst pn2 # node) r));
+    simpl;auto.
+    generalize (is_int_zero_alpha _ _ _ node r H0).
+    intros. rewrite H2. destruct (is_int_zero (nreg (fst pn2 # node) r));simpl;auto.
+    generalize (operation_is_redundant_alpha _ _ _ node r o H0).
+    intros. rewrite H3. destruct (operation_is_redundant o (nreg (fst pn2 # node) r));simpl;auto.
+    destruct l;simpl;auto.
+  - generalize (is_dead_alpha _ _ _ node r H0).
+    intros. rewrite H1. destruct (is_dead (nreg (fst pn2 # node) r));
+    simpl;auto.
+    generalize (is_int_zero_alpha _ _ _ node r H0).
+    intros. rewrite H2. destruct (is_int_zero (nreg (fst pn2 # node) r));simpl;auto.
+  - eapply aaddressing_alpha in H as ?.
+    rewrite H1.
+    erewrite nmem_contains_alpha;auto.
+    destruct (nmem_contains (snd pn2 # node) (aaddressing pva2 # node a0 l) (size_chunk m));simpl;auto.    
+  - destruct s0;simpl;auto.
+  - destruct s0;simpl;auto.
+  - destruct e;simpl;auto.
+    destruct l;simpl;auto.
+    destruct l;simpl;auto.
+    destruct l;simpl;auto.
+    eapply aaddr_arg_alpha in H as ?.
+    rewrite H1.
+    erewrite nmem_contains_alpha;auto.
+    destruct (nmem_contains (snd pn2 # node) (aaddr_arg pva2 # node b0) sz);simpl;auto.
+  - destruct (peq n n0);auto.
+Qed.
+
+
+    
+Lemma transf_function_alpha_aux : forall a code pva1 pva2 pn1 pn2 node,
+    (forall pc, match_VA_alpha a pva1!!pc pva2!!pc) ->
+    (forall pc, match_NA_alpha a pn1!!pc pn2!!pc) ->
+    PTree.xmap (fun (pc : positive) (instr : instruction) => transf_instr pva1 pn1 pc instr) (PTree.map1 (alpha_rename a) code) node =
+          PTree.map1 (alpha_rename a) (PTree.xmap (fun (pc : positive) (instr : instruction) => transf_instr pva2 pn2 pc instr) code node).
+Proof.
+  intros.
+  generalize dependent node.
+  induction code;simpl;auto.
+  intros. destruct o;simpl.
+  - f_equal;auto.
+    f_equal.
+    apply transf_instr_alpha. auto. auto.
+  - f_equal;auto.
+Qed.
+
+  
+Lemma transf_function_alpha: forall a f f' ctx,
+    transf_function (romem_for ctx) f = OK f' ->
+    transf_function (romem_for (alpha_rename a ctx)) (alpha_rename a f) = OK (alpha_rename a f').
+Proof.
+  intros.
+  unfold transf_function in *.
+  generalize (analyze_alpha f a ctx). intros.
+  generalize (Deadcode_analyze_alpha a f _ _ H0). intros.
+  inversion H1.
+  - rewrite <- H4 in H.
+    congruence.
+  - rewrite <- H3 in H.
+    monadInv H.
+    f_equal.
+    Transparent Alpha_function.
+    simpl. unfold alpha_rename_function. simpl.
+    f_equal.
+    unfold PTree.map.
+    assert ({|
+          fn_sig := fn_sig f;
+          fn_params := fn_params f;
+          fn_stacksize := fn_stacksize f;
+          fn_code := PTree.map1 (alpha_rename a) (fn_code f);
+          fn_entrypoint := fn_entrypoint f |} = alpha_rename a f). 
+    { simpl. unfold alpha_rename_function. auto. }
+    simpl in *. rewrite H. clear H.
+    inversion H1.
+    + simpl in *.
+      rewrite <- H5 in H2. congruence.
+    + simpl in *. rewrite <- H in H2. rewrite <- H5 in H3.
+      inversion H2. inversion H3. subst.
+      clear H5 H4 H3 H2 H1 H .
+      apply transf_function_alpha_aux. auto. auto.
+Qed.
+
+Lemma transf_fundef_alpha : forall a fd fd' ctx,
+    transf_fundef (romem_for ctx) fd = OK fd' -> 
+    transf_fundef (romem_for (alpha_rename a ctx)) (alpha_rename a fd) = OK (alpha_rename a fd').
+Proof.
+  unfold transf_fundef.
+  unfold transf_partial_fundef.
+  intros.
+  Transparent Alpha_fundef.
+  destruct fd;destruct fd';simpl in *;try congruence;auto.
+  monadInv H.
+  eapply transf_function_alpha in EQ.
+  rewrite EQ. simpl. auto.
+  monadInv H.
+Qed.
+
+Definition transf_fundef_ctx ctx fd:=
+    transf_fundef (romem_for ctx) fd.
+
+Theorem transf_fundef_ctx_alpha: forall fd fd' a ctx,
+    transf_fundef_ctx ctx fd = OK fd' ->
+    transf_fundef_ctx (alpha_rename a ctx) (alpha_rename a fd) =
+    OK (alpha_rename a fd').
+Proof.
+  intros.
+  unfold transf_fundef_ctx in *.
+  apply transf_fundef_alpha.
+  auto.
+Qed.
